Prove completeness of bisim for trace equivalence.

Equiv/TraceEquiv.v
@@ -36,34 +36,13 @@ Inductive produces_prefix {S} `{StateType S} : S -> list extevent -> Prop :=
       -> step σ evt σ'
       -> produces_prefix σ' L
       -> produces_prefix σ (EEvt evt::L)
-  | producesPrefixTerm (σ:S) (σ':S) v
-    : result σ' = Some v
+  | producesPrefixTerm (σ:S) (σ':S) r
+    : result σ' = r
       -> star2 step σ nil σ'
       -> normal2 step σ'
-      -> produces_prefix σ (EvtTerminate (Some v)::nil)
+      -> produces_prefix σ (EvtTerminate r::nil)
   | producesPrefixPrefix (σ:S)
     : produces_prefix σ nil.
-
-Inductive produces_nondet {S} `{StateType S} : S -> list extevent -> Prop :=
-  | producesNondetSilent (σ:S) (σ':S) L :
-      step σ EvtTau σ'
-      -> produces_nondet σ' L
-      -> produces_nondet σ  L
-  | producesNondetExtern (σ:S) (σ':S) evt L :
-      activated σ
-      -> step σ evt σ'
-      -> produces_nondet σ' L
-      -> produces_nondet σ (EEvt evt::L)
-  | producesNondetTerm (σ:S) (σ':S) v
-    : result σ' = Some v
-      -> star2 step σ nil σ'
-      -> normal2 step σ'
-      -> produces_nondet σ (EvtTerminate (Some v)::nil)
-  | producesNondetPrefix (σ:S) (σ':S) L
-    : result σ' = None
-      -> star2 step σ nil σ'
-      -> normal2 step σ'
-      -> produces_nondet σ L.
 
 Lemma produces_star2_silent {S} `{StateType S} (σ σ':S) L
  : star2 step σ nil σ' ->
@@ -83,15 +62,34 @@ Proof.
     econstructor 1; eauto.
 Qed.
 
-Lemma produces_nondet_star2_silent {S} `{StateType S} (σ σ':S) L
+Lemma star2_reach_silent_step (X : Type) (R:X -> event -> X -> Prop) (x y z : X)
+: R x EvtTau y
+  -> star2 R x nil z
+  -> internally_deterministic R
+  -> x = z \/ star2 R y nil z.
+Proof.
+  intros. inv H0; eauto.
+  exploit H1; eauto. dcr; subst; eauto.
+Qed.
+
+
+Lemma produces_prefix_star2_silent' {S} `{StateType S} (σ σ':S) L
  : star2 step σ nil σ' ->
-   produces_nondet σ' L -> produces_nondet σ L.
+   produces_prefix σ L -> produces_prefix σ' L.
 Proof.
   intros. general induction H0; eauto.
   - destruct yl, y; simpl in *; try congruence.
-    econstructor 1; eauto.
+    eapply IHstar2; eauto.
+    inv H2.
+    + exploit step_internally_deterministic. eapply H. eapply H3.
+      dcr; subst. eauto.
+    + exfalso. inv H3; dcr.
+      exploit step_internally_deterministic. eapply H. eapply H7. dcr; congruence.
+    + exploit star2_reach_silent_step; eauto. eapply H1.
+      destruct X; subst. exfalso. eapply H5; firstorder.
+      econstructor 3; eauto.
+    + econstructor 4.
 Qed.
-
 
 Lemma no_activated_tau_step {S} `{StateType S} (σ σ':S)
  :  activated σ
@@ -132,107 +130,11 @@ Proof.
   eapply bisim_sym; eauto.
 Qed.
 
-
-Lemma sim_produces {S} `{StateType S} {S'} `{StateType S'} (σ:S) (σ':S')
-  : sim σ σ' -> forall L, produces_prefix σ L -> produces_prefix σ' L.
-Proof.
-  intros. general induction H2.
-  - eapply sim_sim' in H3.
-    eapply IHproduces_prefix; eauto.
-    eapply sim'_sim. eapply sim'_reduction_closed_1; eauto.
-    eapply (S_star2 _ _ H0). eapply star2_refl.
-  - eapply sim_sim' in H4.
-    exploit (sim'_activated H0 H4); eauto.
-    destruct X as [? [? [? [?]]]].
-    + destruct evt.
-      * eapply produces_prefix_star2_silent; eauto.
-        edestruct H7; eauto. destruct H9.
-        econstructor 2. eauto. eapply H9.
-        eapply IHproduces_prefix; eauto.
-        eapply sim'_sim. eapply H10.
-      * exfalso; eapply (no_activated_tau_step _ H0 H1); eauto.
-  - eapply sim_sim' in H4. eapply sim'_terminate in H4; eauto.
-    destruct H4 as [? [? []]]. rewrite H0. econstructor 3; [ | eauto | eauto]. congruence.
-    congruence.
-  - eapply producesPrefixPrefix.
-Qed.
-
-
-Lemma sim_produces' {S} `{StateType S} {S'} `{StateType S'} (σ:S) (σ':S')
-  : sim σ σ' -> forall L, produces σ' L -> produces_nondet σ L.
-Proof.
-  intros. general induction H2.
-  - eapply sim_sim' in H3.
-    eapply IHproduces; eauto.
-    eapply sim'_sim. eapply sim'_reduction_closed_2; eauto.
-    eapply (S_star2 _ _ H). eapply star2_refl.
-  - eapply sim_sim' in H4.
-    exploit (sim'_activated_2 H H4); eauto.
-    destruct X as [? [? [[? []]|]]].
-    + destruct evt.
-      * eapply produces_nondet_star2_silent; eauto.
-        edestruct H7; eauto. destruct H9.
-        econstructor 2. eauto. eapply H9.
-        eapply IHproduces; eauto.
-        eapply sim'_sim. eapply H10.
-      * exfalso; eapply (no_activated_tau_step _ H H1); eauto.
-    + dcr. econstructor 4; eauto.
-  - eapply sim_sim' in H4. eapply sim'_terminate_2 in H4; eauto; try congruence.
-    destruct H4 as [? [? [? [|]]]].
-    + case_eq (result σ'); intros.
-      * econstructor 3; [ | eauto | eauto]. congruence.
-      * eapply producesNondetPrefix; eauto. congruence.
-    + eapply producesNondetPrefix; eauto.
-Qed.
-
 CoInductive diverges S `{StateType S} : S -> Prop :=
 | DivergesI σ σ'
   : step σ EvtTau σ'
     -> diverges σ'
     -> diverges σ.
-
-CoInductive diverges_gen S `{StateType S} (r:S -> Prop) : S -> Prop :=
-| DivergesGenI σ σ'
-  : step σ EvtTau σ'
-    -> r σ'
-    -> diverges_gen r σ.
-
-Hint Constructors diverges_gen.
-
-Definition diverges' S `{StateType S} : S -> Prop :=
-  paco1 (@diverges_gen S _) bot1.
-
-Hint Unfold diverges'.
-
-Lemma diverges_gen_mon S `{StateType S}
-: monotone1 (@diverges_gen S _).
-Proof.
-  hnf; intros. inv IN.
-  - econstructor 1; eauto.
-Qed.
-
-Hint Resolve diverges_gen_mon : paco.
-
-Lemma diverges_diverges' S `{StateType S} (σ:S)
-: diverges σ -> diverges' σ.
-Proof.
-  revert σ. pcofix CIH.
-  intros. pfold.
-  inv H1.
-  econstructor; eauto.
-Qed.
-
-Lemma diverges'_diverges S `{StateType S} (σ:S)
-  : diverges' σ -> diverges σ.
-Proof.
-  revert σ.
-  cofix COH; intros.
-  assert (diverges_gen (paco1 (diverges_gen (S:=S)) bot1 \1/ bot1) σ).
-  punfold H0.
-  inv H1.
-  econstructor; eauto.
-  destruct H3; eauto. inv H3.
-Qed.
 
 Lemma diverges_reduction_closed S `{StateType S} (σ σ':S)
 : diverges σ -> star2 step σ nil σ'  -> diverges σ'.
@@ -279,6 +181,15 @@ Proof.
     + eapply H2.
 Qed.
 
+Lemma bisim_complete_diverges S `{StateType S} S' `{StateType S'} (σ:S) (σ':S')
+: diverges σ -> diverges σ' -> bisim σ σ'.
+Proof.
+  revert σ σ'. cofix COH; intros.
+  inv H1; inv H2.
+  econstructor. econstructor; eauto. econstructor; eauto.
+  eapply COH; eauto.
+Qed.
+
 CoInductive stream (A : Type) : Type :=
 | sil : stream A
 | sons : A -> stream A -> stream A.
@@ -290,7 +201,7 @@ CoInductive coproduces {S} `{StateType S} : S -> stream extevent -> Prop :=
     star2 step σ nil σ'
       -> activated σ'
       -> step σ' evt σ''
-      -> coproduces σ' L
+      -> coproduces σ'' L
       -> coproduces σ (sons (EEvt evt) L)
 | CoProducesSilent (σ:S) :
     diverges σ
@@ -325,7 +236,7 @@ Proof.
   eapply coproduces_reduction_closed_step; eauto.
 Qed.
 
-Lemma bisim_coproduces {S} `{StateType S} {S'} `{StateType S'} (sigma:S) (σ':S')
+Lemma bisim_coproduces S `{StateType S} S' `{StateType S'} (sigma:S) (σ':S')
   : bisim sigma σ' -> forall L, coproduces sigma L -> coproduces σ' L.
 Proof.
   revert sigma σ'. cofix COH; intros.
@@ -337,13 +248,242 @@ Proof.
     edestruct H10. eauto. dcr.
     econstructor; try eapply H8. eauto. eapply H11.
     eapply COH; eauto.
-    eapply bisim'_bisim. eapply (bisim'_reduction_closed H7); eauto.
-    econstructor.
+    destruct H11.
+    eapply bisim'_bisim. eapply H13.
   - econstructor. eapply (bisim_sound_diverges H1); eauto.
   - exploit (bisim'_terminate H4 H5 (bisim_bisim' H1)).
     dcr.
     econstructor; eauto.
 Qed.
+
+Lemma produces_only_nil_diverges S `{StateType S} (σ:S)
+: (forall L, produces_prefix σ L -> L = nil) -> diverges σ.
+Proof.
+  revert σ. cofix f; intros.
+  destruct (@step_dec _ H σ).
+  - destruct H1; dcr. destruct x.
+    + exfalso. exploit H0. econstructor 2; try eapply H2.
+      eexists; eauto.
+      econstructor 4. congruence.
+    + econstructor. eauto. eapply f.
+      intros. eapply H0.
+      eapply produces_prefix_star2_silent.
+      eapply (S_star2 EvtTau); eauto. econstructor. eauto.
+  - exfalso.
+    exploit H0. econstructor 3. reflexivity. econstructor. eauto. congruence.
+Qed.
+
+Lemma produces_prefix_extevent S `{StateType S} (σ:S) evt L
+: produces_prefix σ (EEvt evt::L)
+  -> exists σ', star2 step σ nil σ'
+          /\ activated σ'
+          /\ exists σ'', step σ' evt σ'' /\ produces_prefix σ'' L.
+Proof.
+  intros. general induction H0.
+  - edestruct IHproduces_prefix. reflexivity. dcr.
+    eexists x; intuition. eapply (S_star2 EvtTau); eauto.
+    eexists; eauto.
+  - eexists σ; intuition. econstructor. eexists; eauto.
+Qed.
+
+Lemma produces_prefix_terminates S `{StateType S} (σ:S) r L
+:  produces_prefix σ (EvtTerminate r::L)
+   -> exists σ', star2 step σ nil σ' /\ normal2 step σ' /\ result σ' = r /\ L = nil.
+Proof.
+  intros. general induction H0.
+  - edestruct IHproduces_prefix. reflexivity.
+    eexists x; dcr; intuition. eapply (S_star2 EvtTau); eauto.
+  - eexists; intuition; eauto.
+Qed.
+
+Lemma diverges_produces_only_nil S `{StateType S} S' `{StateType S'} (σ:S)
+: diverges σ -> (forall L, produces_prefix σ L -> L = nil).
+Proof.
+  intros. general induction L; eauto.
+  destruct a.
+  - eapply produces_prefix_extevent in H2; dcr.
+    exfalso. eapply diverges_never_activated; eauto.
+    eapply diverges_reduction_closed; eauto.
+  - eapply produces_prefix_terminates in H2; dcr; subst.
+    exfalso. eapply diverges_never_terminates; eauto using diverges_reduction_closed.
+Qed.
+
+Lemma produces_diverges S `{StateType S} S' `{StateType S'} (σ:S) (σ':S')
+: (forall L, produces_prefix σ L <-> produces_prefix σ' L)
+  -> diverges σ -> diverges σ'.
+Proof.
+  revert σ σ'.
+  cofix f; intros.
+  inv H2.
+  edestruct (@step_dec _ H0 σ').
+  inv H5; dcr.
+  destruct x.
+  - exfalso.
+    pose proof (diverges_produces_only_nil H2).
+    exploit H6. eapply H1.
+    econstructor 2. eexists; eauto. eauto. econstructor 4.
+    congruence.
+  - econstructor. eapply H7.
+    eapply f; intros; try eapply H4.
+    split; intros.
+    + eapply produces_prefix_star2_silent'.
+      eapply (S_star2 EvtTau). eapply H7. econstructor.
+      eapply H1. econstructor; eauto.
+    + eapply produces_prefix_star2_silent'.
+      eapply (S_star2 EvtTau). eapply H3. econstructor.
+      eapply H1. econstructor; eauto.
+  - exfalso.
+    exploit (diverges_produces_only_nil H2).
+    eapply H1. econstructor 3; eauto. constructor.
+    congruence.
+Qed.
+
+Lemma produces_prefix_star_activated S `{StateType S} (σ1 σ1' σ1'':S) evt L
+: star2 step σ1 nil σ1'
+  -> activated σ1'
+  -> step σ1' evt σ1''
+  -> produces_prefix σ1'' L
+  -> produces_prefix σ1 (EEvt evt::L).
+Proof.
+  intros. general induction H0.
+  - econstructor 2; eauto.
+  - destruct y, yl; simpl in *; try congruence.
+    econstructor; eauto.
+Qed.
+
+Lemma produces_prefix_preserved' S `{StateType S} S' `{StateType S'} (σ1 σ1' σ1'':S) (σ2 σ2' σ2'':S') evt
+: (forall L : list extevent, produces_prefix σ1 L <-> produces_prefix σ2 L)
+  -> star2 step σ1 nil σ1'
+  -> activated σ1'
+  -> step σ1' evt σ1''
+  -> star2 step σ2 nil σ2'
+  -> activated σ2'
+  -> step σ2' evt σ2''
+  -> forall L, produces_prefix σ1'' L -> produces_prefix σ2'' L.
+Proof.
+  intros.
+  - exploit (produces_prefix_star_activated _ H2 H3 H4 H8).
+    eapply H1 in X.
+    eapply produces_prefix_extevent in X. dcr.
+    exploit both_activated. eapply H10. eapply H5. eauto. eauto. subst.
+    assert (x0 = σ2''). eapply step_externally_determined; eauto. subst; eauto.
+Qed.
+
+
+Lemma produces_prefix_preserved S `{StateType S} S' `{StateType S'} (σ1 σ1' σ1'':S) (σ2 σ2' σ2'':S') evt
+:
+  (forall L : list extevent, produces_prefix σ1 L <-> produces_prefix σ2 L)
+  -> star2 step σ1 nil σ1'
+  -> activated σ1'
+  -> step σ1' evt σ1''
+  -> star2 step σ2 nil σ2'
+  -> activated σ2'
+  -> step σ2' evt σ2''
+  -> forall L, produces_prefix σ1'' L <-> produces_prefix σ2'' L.
+Proof.
+  split; intros.
+  eapply (produces_prefix_preserved' _ _ H1); eauto.
+  symmetry in H1.
+  eapply (produces_prefix_preserved' _ _ H1); eauto.
+Qed.
+
+Lemma produces_coproduces S `{StateType S} S' `{StateType S'} (σ:S) (σ':S')
+: (forall L, produces_prefix σ L <-> produces_prefix σ' L)
+  -> (forall T, coproduces σ T -> coproduces σ' T).
+Proof.
+  revert σ σ'.
+  cofix f; intros.
+  inv H2.
+  - assert (produces_prefix σ (EEvt evt::nil)).
+    eapply produces_prefix_star_activated; eauto. econstructor 4.
+    eapply H1 in H7.
+    eapply produces_prefix_extevent in H7. dcr.
+    econstructor. eauto. eauto. eauto. eapply f; try eapply H6.
+    eapply (produces_prefix_preserved _ _ _ H1); eauto.
+  - exploit (produces_diverges H1 H3).
+    econstructor. eauto.
+  - assert (produces_prefix σ (EvtTerminate (result σ'0)::nil)).
+    econstructor 3; eauto. eapply H1 in H3.
+    eapply produces_prefix_terminates in H3. dcr.
+    econstructor 3; eauto.
+Qed.
+
+Require Import Classical_Prop.
+
+Lemma three_possibilities S `{StateType S} (σ:S)
+: (exists σ', star2 step σ nil σ' /\ normal2 step σ')
+  \/ (exists σ', star2 step σ nil σ' /\ activated σ')
+  \/ diverges σ.
+Proof.
+  destruct (classic (exists σ' : S, star2 step σ nil σ' /\ normal2 step σ')); intuition; right.
+  destruct (classic (exists σ' : S, star2 step σ nil σ' /\ activated σ')); intuition; right.
+  revert σ H0 H1. cofix f.
+  intros. destruct (@step_dec _ H σ). inv H2; dcr.
+  destruct x.
+  - exfalso. eapply H1; eexists σ; intuition.
+    econstructor. do 2 eexists; eauto.
+  - econstructor. eauto. eapply f; intros; dcr.
+    eapply H0; eexists; split; eauto. eapply (S_star2 EvtTau); eauto.
+    eapply H1; eexists; split; eauto. eapply (S_star2 EvtTau); eauto.
+  - exfalso. eapply H0; eexists σ; intuition. econstructor.
+Qed.
+
+Lemma produces_silent_closed {S} `{StateType S}  S' `{StateType S'}  (σ1 σ1':S) (σ2 σ2':S')
+: star2 step σ1 nil σ1'
+  -> star2 step σ2 nil σ2'
+  -> (forall L, produces_prefix σ1 L <-> produces_prefix σ2 L)
+  -> (forall L, produces_prefix σ1' L <-> produces_prefix σ2' L).
+Proof.
+  split; intros.
+  - eapply produces_prefix_star2_silent'; eauto. eapply H3.
+    eapply produces_prefix_star2_silent; eauto.
+  - eapply produces_prefix_star2_silent'; eauto. eapply H3.
+    eapply produces_prefix_star2_silent; eauto.
+Qed.
+
+Lemma produces_prefix_bisim S `{StateType S} S' `{StateType S'} (σ:S) (σ':S')
+: (forall L, produces_prefix σ L <-> produces_prefix σ' L)
+  -> bisim σ σ'.
+Proof.
+  revert σ σ'.
+  cofix f; intros.
+  destruct (three_possibilities σ) as [A|[A|A]].
+  - dcr. assert (produces_prefix σ (EvtTerminate (result x)::nil)).
+    econstructor 3; eauto.
+    eapply H1 in H2.
+    eapply produces_prefix_terminates in H2. dcr.
+    econstructor 3; eauto.
+  - dcr. inv H4; dcr.
+    assert (produces_prefix x1 nil) by econstructor 4.
+    exploit (produces_prefix_star_activated _ H3 H4 H5 H2).
+    eapply H1 in X.
+    eapply produces_prefix_extevent in X. dcr.
+    econstructor 2; eauto.
+    + intros.
+      assert (B:produces_prefix x (EEvt evt::nil)) by
+          (econstructor 2; eauto; econstructor 4).
+      pose proof H1.
+      eapply produces_silent_closed in H11; eauto.
+      eapply H11 in B.
+      inv B.
+      * exfalso. exploit (step_internally_deterministic _ _ _ _ H12 H9 ); eauto. dcr; congruence.
+      * eexists; split. eauto. eapply f.
+        eapply produces_prefix_preserved; eauto.
+    + intros.
+      assert (B:produces_prefix x2 (EEvt evt::nil)) by
+          (econstructor 2; eauto; econstructor 4).
+      pose proof H1.
+      eapply produces_silent_closed in H11; eauto.
+      eapply H11 in B.
+      inv B.
+      * exfalso. exploit (step_internally_deterministic _ _ _ _ H12 H5 ); eauto. dcr; congruence.
+      * eexists; split. eauto. eapply f.
+        eapply produces_prefix_preserved; eauto.
+  - assert (diverges σ').
+    eapply (produces_diverges H1); eauto.
+    eapply bisim_complete_diverges; eauto.
+Qed.
+
 
 
 
